Updates.

FOL/NV/Definition.lean
@@ -35,19 +35,19 @@ deriving DecidableEq
 /--
   The type of environments.
 -/
-def Env : Type := List Definition_
+def Env_ : Type := List Definition_
 
-instance : Membership Definition_ Env :=
+instance : Membership Definition_ Env_ :=
   inferInstanceAs (Membership Definition_ (List Definition_))
 
-instance : HAppend Env Env Env :=
+instance : HAppend Env_ Env_ Env_ :=
   inferInstanceAs (HAppend (List Definition_) (List Definition_) (List Definition_))
 
 
 /--
   `Formula_.all_def_in_env E F` := True if and only if every definition that occurs in the formula `F` is in the environment `E`.
 -/
-def Formula_.all_def_in_env (E : Env) : Formula_ → Prop
+def Formula_.all_def_in_env (E : Env_) : Formula_ → Prop
 | pred_const_ _ _ => True
 | pred_var_ _ _ => True
 | eq_ _ _ => True
@@ -71,7 +71,7 @@ def Formula_.all_def_in_env (E : Env) : Formula_ → Prop
 | def_ X xs =>
   ∃ (d : Definition_), d ∈ E ∧ X = d.name ∧ xs.length = d.args.length
 
-instance (E : Env) (F : Formula_) : Decidable (F.all_def_in_env E) :=
+instance (E : Env_) (F : Formula_) : Decidable (F.all_def_in_env E) :=
   by
   induction F
   all_goals
@@ -80,36 +80,36 @@ instance (E : Env) (F : Formula_) : Decidable (F.all_def_in_env E) :=
 
 
 /--
-  `Env.nodup_ E` := True if and only if every definition that occurs in the environment `E` has a unique combination of name and argument length.
+  `Env_.nodup_ E` := True if and only if every definition that occurs in the environment `E` has a unique combination of name and argument length.
 -/
-def Env.nodup_ : Env → Prop :=
+def Env_.nodup_ : Env_ → Prop :=
   List.Pairwise (fun (d1 d2 : Definition_) => d1.name = d2.name → d1.args.length = d2.args.length → False)
 
-instance (E : Env) : Decidable (E.nodup_) :=
+instance (E : Env_) : Decidable (E.nodup_) :=
   by
   induction E
   all_goals
-    simp only [Env.nodup_]
+    simp only [Env_.nodup_]
     infer_instance
 
 
 /--
-  `Env.well_formed E` := True if and only if
+  `Env_.well_formed E` := True if and only if
   1. Every definition that occurs in the environment `E` has a unique combination of name and argument length.
   2. Every definition that occurs in the formula of a definition `d` in the environment `d :: E' ⊆ E` occurs in the environment `E'`. This means there are no circular definitions.
 -/
-def Env.well_formed : Env → Prop
+def Env_.well_formed : Env_ → Prop
   | List.nil => True
   | d :: E =>
     (∀ (d' : Definition_), d' ∈ E →
       d.name = d'.name → d.args.length = d'.args.length → False) ∧
-        Formula_.all_def_in_env E d.q ∧ Env.well_formed E
+        Formula_.all_def_in_env E d.q ∧ Env_.well_formed E
 
-instance (E : Env) : Decidable (E.well_formed) :=
+instance (E : Env_) : Decidable (E.well_formed) :=
   by
   induction E
   all_goals
-    simp only [Env.well_formed]
+    simp only [Env_.well_formed]
     infer_instance
 
 
