FOL/NV/Sub/Pred/All/Rec/Sub.lean
@@ -110,7 +110,7 @@ theorem substitution_theorem_aux
   (D : Type)
   (I : Interpretation_ D)
   (V V' : Valuation_ D)
-  (E : Env)
+  (E : Env_)
   (τ : PredName_ → ℕ → List VarName_ × Formula_)
   (binders : Finset VarName_)
   (F : Formula_)
@@ -242,7 +242,7 @@ theorem substitution_theorem
   (D : Type)
   (I : Interpretation_ D)
   (V : Valuation_ D)
-  (E : Env)
+  (E : Env_)
   (τ : PredName_ → ℕ → List VarName_ × Formula_)
   (F : Formula_)
   (h1 : admits τ F) :
