FOL/NV/Sub/Var/All/Rec/Admits.lean
@@ -75,7 +75,7 @@ theorem substitution_theorem_aux
   (D : Type)
   (I : Interpretation_ D)
   (V V' : Valuation_ D)
-  (E : Env)
+  (E : Env_)
   (σ σ' : VarName_ → VarName_)
   (binders : Finset VarName_)
   (F : Formula_)
@@ -210,7 +210,7 @@ theorem substitution_theorem
   (D : Type)
   (I : Interpretation_ D)
   (V : Valuation_ D)
-  (E : Env)
+  (E : Env_)
   (σ : VarName_ → VarName_)
   (F : Formula_)
   (h1 : admits σ F) :
